\par In an orthnormal basis $\{\ket{i}\}$,

\begin{align}
\mathrm{tr} \left( \ket{\alpha} \bra{\beta} \right) &= \mathrm{tr} \left[ \left(
\sum_i{a_i \ket{i}} \right) \left( \sum_j{b_j^* \bra{j}} \right) \right] \\
&= \mathrm{tr} \left( \sum_{i, j}{a_i b_j^* \ket{i} \bra{j}} \right) \\
&= \sum_{i, j}{a_i b_j^* \mathrm{tr} \left( \ket{i} \bra{j} \right)} \\
&= \sum_{i, j}{a_i b_j^* \delta_{ij}} = \braket{\beta|\alpha}
\end{align}

\par Now let $\rho = \sum_i{p_i \ket{\psi_i} \bra{\psi_i}}$ be a density
operator where $\{\ket{\psi_i}\}$ are all normal but may not necessarily be
orthogonal to each other. Then, $\rho^2 = \sum_{i, j}{p_i p_j
\braket{\psi_i|\psi_j} \ket{\psi_i} \bra{\psi_j}}$ and:

\begin{align}
\mathrm{tr} \left( \rho^2 \right) &= \sum_{i, j}{p_i p_j \mathrm{tr} \left(
\ket{\psi_i} \bra{\psi_j} \right)} \\
&= \sum_{i \ne j}{p_i p_j \mathrm{tr} \left( \ket{\psi_i} \bra{\psi_j} \right)}
+ \sum_k{p_k^2 \mathrm{tr} \left( \ket{\psi_k} \bra{\psi_k} \right)} \\
&= \sum_{i \ne j}{p_i p_j \braket{\psi_j|\psi_i}} + \sum_k{p_k^2
\braket{\psi_k|\psi_k}} \\
&\le \sum_{i \ne j}{p_i p_j} + \sum_k{p_k^2} \\
&= \left( \sum_i{p_i} \right)^2 = 1
\end{align}

\par In a pure state, $p_r = 1$ for some fixed $r$ and necessarily, all other
$p_i = 0$ (thus, $p_i p_r = \delta_{ir}$). Then:

\begin{align}
\mathrm{tr} \left( \rho^2 \right) &= \sum_{i \ne j}{p_i p_j
\braket{\psi_j|\psi_i}} + \sum_k{p_k^2 \braket{\psi_k|\psi_k}} \\
&= \sum_k{p_k^2 \braket{\psi_k|\psi_k}} \\
&= p_r^2 \braket{\psi_r|\psi_r} = 1^2 \cdot 1 = 1
\end{align}

\par Conversely, suppose that $\mathrm{tr} \left( \rho^2 \right) = 1$. Then,

\begin{align}
\sum_{i \ne j}{p_i p_j \braket{\psi_j|\psi_i}} + \sum_k{p_k^2
\braket{\psi_k|\psi_k}} &= 1 \\
\sum_{i \ne j}{p_i p_j \braket{\psi_j|\psi_i}} + \sum_k{p_k^2} &= \left(
\sum_k{p^k} \right)^2 = \sum_{i \ne j}{p_i p_j} + \sum_k{p_k^2} \\
\sum_{i \ne j}{p_i p_j \braket{\psi_j|\psi_i}} &= \sum_{i \ne j}{p_i p_j} \\
p_i p_j \braket{\psi_j|\psi_i} &= p_i p_j, \quad i \ne j
\end{align}

Suppose that there exists a pair $r \ne s$ such that $p_r p_s > 0$. Then:

$$
p_r p_s \braket{\psi_s|\psi_r} = p_r p_s \Rightarrow \braket{\psi_s|\psi_r} = 1
\Rightarrow \ket{\psi_r} = \ket{\psi_s} \Rightarrow r = s
$$

leading to a contradiction. So the product of probabilities for every pair of
distinct states must be zero, which means that there can be at most one non-zero
$p_r$.  They cannot all be zero either, because $\sum_k{p_k} = 1$. Thus,
$\sum_k{p_k} = p_r = 1$.
